Prove `itree_machine_semantics`
Expresses `machine_sem` in terms of itree target semantics

cakeml-semantics/target_semanticsProofScript.sml
@@ -265,6 +265,799 @@ Proof
     )
 QED
 
+
+(*********** halt_rel **********)
+
+Definition halt_rel_def:
+  halt_rel Termination h = (h = Success) ∧
+  halt_rel OutOfMemory h = (h = Resource_limit_hit) ∧
+  halt_rel _ _ = F
+End
+
+Triviality halt_rel_alt_def:
+  halt_rel h Success = (h = Termination) ∧
+  halt_rel h Resource_limit_hit = (h = OutOfMemory) ∧
+  halt_rel h (FFI_outcome _) = F
+Proof
+  Cases_on `h` >> rw[halt_rel_def]
+QED
+
+Triviality halt_rel_imps:
+  halt_rel r h ⇒ r ≠ Error ∧ (∀p out. r ≠ FinalFFI p out)
+Proof
+  rw[] >> CCONTR_TAC >> gvs[halt_rel_def]
+QED
+
+
+(*********** eval_to' / evaluate' - non-FFI steps **********)
+
+Theorem eval_to'_evaluate'_halt_rel:
+  halt_rel r h ⇒ (
+  eval_to' k mc ms = (Ret' r,mc',ms') ⇔
+  evaluate' mc (ffi :'ffi ffi_state) k ms = (Halt h,mc',ms',ffi))
+Proof
+  rw[] >> imp_res_tac halt_rel_imps >>
+  eq_tac >> rw[] >> pop_assum mp_tac
+  >- (
+    map_every qid_spec_tac [`ffi`,`ms`,`mc`,`k`] >>
+    ho_match_mp_tac eval_to'_ind >> rw[] >>
+    pop_assum mp_tac >> simp[Once eval_to'_def, Once evaluate'_def] >>
+    IF_CASES_TAC >> gvs[] >> IF_CASES_TAC >> gvs[]
+    >- (IF_CASES_TAC >> gvs[] >> pairarg_tac >> gvs[] >> IF_CASES_TAC >> gvs[])
+    >- (
+      IF_CASES_TAC >> gvs[] >- (rw[] >> gvs[halt_rel_def]) >>
+      IF_CASES_TAC >> gvs[] >- (pairarg_tac >> gvs[]) >>
+      ntac 5 (TOP_CASE_TAC >> gvs[]) >>
+      strip_tac >> gvs[call_FFI_def, apply_oracle_def]
+      )
+    )
+  >- (
+    map_every qid_spec_tac [`ms`,`k`,`ffi`,`mc`] >>
+    ho_match_mp_tac evaluate'_ind >> rw[] >>
+    pop_assum mp_tac >> simp[Once eval_to'_def, Once evaluate'_def] >>
+    IF_CASES_TAC >> gvs[] >> IF_CASES_TAC >> gvs[]
+    >- (IF_CASES_TAC >> gvs[] >> pairarg_tac >> gvs[] >> IF_CASES_TAC >> gvs[])
+    >- (
+      IF_CASES_TAC >> gvs[] >- (rw[] >> Cases_on `r` >> gvs[halt_rel_def]) >>
+      IF_CASES_TAC >> gvs[] >- (pairarg_tac >> gvs[]) >>
+      reverse $ ntac 5 (TOP_CASE_TAC >> gvs[])
+      >- (strip_tac >> gvs[] >> Cases_on `r` >> gvs[halt_rel_def]) >>
+      strip_tac >> gvs[apply_oracle_def] >>
+      qsuff_tac `ffi = f`
+      >- (strip_tac >> gvs[call_FFI_def, AllCaseEqs(), ffi_state_component_equality]) >>
+      irule io_events_mono_antisym >>
+      imp_res_tac evaluate'_io_events_mono >> simp[] >>
+      irule call_FFI_rel_io_events_mono >> irule RTC_SUBSET >>
+      simp[call_FFI_rel_def, SF SFY_ss]
+      )
+    )
+QED
+
+Theorem eval_to'_evaluate'_error:
+  eval_to' k mc ms = (Ret' Error,mc',ms') ⇔
+  evaluate' mc (ffi :'ffi ffi_state) k ms = (Error,mc',ms', ffi)
+Proof
+  eq_tac >> rw[] >> pop_assum mp_tac
+  >- (
+    map_every qid_spec_tac [`ffi`,`ms`,`mc`,`k`] >>
+    ho_match_mp_tac eval_to'_ind >> rw[] >>
+    pop_assum mp_tac >> simp[Once eval_to'_def, Once evaluate'_def] >>
+    IF_CASES_TAC >> gvs[] >> IF_CASES_TAC >> gvs[]
+    >- (IF_CASES_TAC >> gvs[] >> pairarg_tac >> gvs[] >> IF_CASES_TAC >> gvs[])
+    >- (
+      IF_CASES_TAC >> gvs[] >- rw[] >>
+      IF_CASES_TAC >> gvs[] >- (pairarg_tac >> gvs[]) >>
+      ntac 5 (TOP_CASE_TAC >> gvs[]) >>
+      strip_tac >> gvs[call_FFI_def, apply_oracle_def]
+      )
+    )
+  >- (
+    map_every qid_spec_tac [`ms`,`k`,`ffi`,`mc`] >>
+    ho_match_mp_tac evaluate'_ind >> rw[] >>
+    pop_assum mp_tac >> simp[Once eval_to'_def, Once evaluate'_def] >>
+    IF_CASES_TAC >> gvs[] >> IF_CASES_TAC >> gvs[]
+    >- (IF_CASES_TAC >> gvs[] >> pairarg_tac >> gvs[] >> IF_CASES_TAC >> gvs[])
+    >- (
+      IF_CASES_TAC >> gvs[] >- (rw[] >> CCONTR_TAC >> gvs[]) >>
+      IF_CASES_TAC >> gvs[] >- (pairarg_tac >> gvs[]) >>
+      ntac 5 (TOP_CASE_TAC >> gvs[]) >>
+      strip_tac >> gvs[apply_oracle_def] >>
+      qsuff_tac `ffi = f`
+      >- (strip_tac >> gvs[call_FFI_def, AllCaseEqs(), ffi_state_component_equality]) >>
+      irule io_events_mono_antisym >>
+      imp_res_tac evaluate'_io_events_mono >> simp[] >>
+      irule call_FFI_rel_io_events_mono >> irule RTC_SUBSET >>
+      simp[call_FFI_rel_def, SF SFY_ss]
+      )
+    )
+QED
+
+Theorem eval_to'_evaluate'_timeout:
+  eval_to' k mc ms = (Div',mc',ms') ⇔
+  evaluate' mc (ffi :'ffi ffi_state) k ms = (TimeOut,mc',ms',ffi)
+Proof
+  eq_tac >> rw[] >> pop_assum mp_tac
+  >- (
+    map_every qid_spec_tac [`ffi`,`ms`,`mc`,`k`] >>
+    ho_match_mp_tac eval_to_ind >> rw[] >>
+    pop_assum mp_tac >> simp[Once eval_to'_def, Once evaluate'_def] >>
+    IF_CASES_TAC >> gvs[] >> IF_CASES_TAC >> gvs[]
+    >- (IF_CASES_TAC >> gvs[] >> pairarg_tac >> gvs[] >> IF_CASES_TAC >> gvs[])
+    >- (
+      IF_CASES_TAC >> gvs[] >- rw[] >>
+      IF_CASES_TAC >> gvs[] >- (pairarg_tac >> gvs[]) >>
+      ntac 5 (TOP_CASE_TAC >> gvs[]) >>
+      strip_tac >> gvs[call_FFI_def, apply_oracle_def]
+      )
+    )
+  >- (
+    map_every qid_spec_tac [`ms`,`k`,`ffi`,`mc`] >>
+    ho_match_mp_tac evaluate_ind >> rw[] >>
+    pop_assum mp_tac >> simp[Once eval_to'_def, Once evaluate'_def] >>
+    IF_CASES_TAC >> gvs[] >> IF_CASES_TAC >> gvs[]
+    >- (IF_CASES_TAC >> gvs[] >> pairarg_tac >> gvs[] >> IF_CASES_TAC >> gvs[])
+    >- (
+      IF_CASES_TAC >> gvs[] >- (rw[] >> CCONTR_TAC >> gvs[]) >>
+      IF_CASES_TAC >> gvs[] >- (pairarg_tac >> gvs[]) >>
+      ntac 5 (TOP_CASE_TAC >> gvs[]) >>
+      strip_tac >> gvs[apply_oracle_def] >>
+      qsuff_tac `ffi = f`
+      >- (strip_tac >> gvs[call_FFI_def, AllCaseEqs(), ffi_state_component_equality]) >>
+      irule io_events_mono_antisym >>
+      imp_res_tac evaluate'_io_events_mono >> simp[] >>
+      irule call_FFI_rel_io_events_mono >> irule RTC_SUBSET >>
+      simp[call_FFI_rel_def, SF SFY_ss]
+      )
+    )
+QED
+
+
+(*********** eval / evaluate - non-FFI steps **********)
+
+Theorem eval_evaluate_halt_rel:
+  halt_rel r h ⇒ (
+  eval (mc,ms) = Ret' r ⇔
+  ∃k ms'. evaluate mc (ffi :'ffi ffi_state) k ms = (Halt h, ms', ffi))
+Proof
+  rw[] >> simp[eval_def] >> DEEP_INTRO_TAC some_intro >> reverse $ rw[] >>
+  gvs[eval_to_eval_to', evaluate_evaluate']
+  >- (
+    CCONTR_TAC >> gvs[] >> pairarg_tac >> gvs[] >>
+    drule_all $ SRULE [PULL_EXISTS] $ iffRL eval_to'_evaluate'_halt_rel >> rw[] >>
+    first_x_assum $ qspec_then `k` assume_tac >> gvs[] >>
+    Cases_on `eval_to' k mc ms` >> gvs[]
+    ) >>
+  eq_tac >> rw[]
+  >- (
+    qmatch_asmsub_abbrev_tac `FST res = _` >> PairCases_on `res` >> gvs[] >>
+    drule_all $ iffLR eval_to'_evaluate'_halt_rel >>
+    rw[] >> qexists_tac `x` >> pairarg_tac >> gvs[]
+    )
+  >- (
+    pairarg_tac >> gvs[] >>
+    drule_all $ SRULE [PULL_EXISTS] $ iffRL eval_to'_evaluate'_halt_rel >> rw[] >>
+    dxrule eval_to'_agree >> simp[] >> disch_then drule >>
+    disch_then $ assume_tac o GSYM >> gvs[]
+    )
+QED
+
+Theorem eval_evaluate_error:
+  eval (mc,ms) = Ret' Error ⇔
+  ∃k ms'. evaluate mc (ffi :'ffi ffi_state) k ms = (Error, ms', ffi)
+Proof
+  rw[] >> simp[eval_def] >> DEEP_INTRO_TAC some_intro >> reverse $ rw[] >>
+  gvs[eval_to_eval_to', evaluate_evaluate']
+  >- (
+    CCONTR_TAC >> gvs[] >> pairarg_tac >> gvs[] >>
+    drule_all $ SRULE [PULL_EXISTS] $ iffRL eval_to'_evaluate'_error >> rw[] >>
+    first_x_assum $ qspec_then `k` assume_tac >> gvs[] >>
+    Cases_on `eval_to' k mc ms` >> gvs[]
+    ) >>
+  eq_tac >> rw[]
+  >- (
+    qmatch_asmsub_abbrev_tac `FST res = _` >> PairCases_on `res` >> gvs[] >>
+    drule_all $ iffLR eval_to'_evaluate'_error >>
+    rw[] >> qexists_tac `x` >> pairarg_tac >> gvs[]
+    )
+  >- (
+    pairarg_tac >> gvs[] >>
+    drule_all $ SRULE [PULL_EXISTS] $ iffRL eval_to'_evaluate'_error >> rw[] >>
+    drule eval_to'_agree >> simp[] >> disch_then drule >>
+    disch_then $ assume_tac o GSYM >> gvs[]
+    )
+QED
+
+Theorem eval_evaluate_timeout:
+  eval (mc,ms) = Div' ⇔
+  ∀k. ∃ms'. evaluate mc (ffi :'ffi ffi_state) k ms = (TimeOut, ms', ffi)
+Proof
+  eq_tac >> simp[eval_def] >> DEEP_INTRO_TAC some_intro >> rw[] >>
+  gvs[eval_to_eval_to', evaluate_evaluate']
+  >- (
+    pairarg_tac >> gvs[] >>
+    first_x_assum $ qspec_then `k` assume_tac >>
+    qmatch_asmsub_abbrev_tac `FST res` >> PairCases_on `res` >> gvs[] >>
+    imp_res_tac eval_to'_evaluate'_timeout >> gvs[]
+    )
+  >- (
+    CCONTR_TAC >> gvs[] >> last_x_assum mp_tac >> simp[] >>
+    first_x_assum $ qspec_then `x` assume_tac >> pairarg_tac >> gvs[] >>
+    imp_res_tac eval_to'_evaluate'_timeout >> gvs[]
+    )
+QED
+
+
+(*********** eval_to' / evaluate' - FFI steps **********)
+
+Theorem evaluate'_1_ffi_changed_eval_to':
+  evaluate' mc (ffi:'ffi ffi_state) 1 ms = (res,mc',ms',ffi') ∧ ffi' ≠ ffi ⇒
+  ∃s conf ws f ms''. eval_to' 1 mc ms = (Vis' (s,conf,ws) f,mc',ms'')
+Proof
+  rw[evaluate'_1_ffi_changed, eval_to'_1_Vis] >> simp[SF SFY_ss]
+QED
+
+Theorem evaluate'_1_ffi_failed_eval_to':
+  evaluate' mc (ffi:'ffi ffi_state) 1 ms = (Halt (FFI_outcome outcome),mc',ms',ffi') ⇒
+  ∃s conf ws f mc''. eval_to' 1 mc ms = (Vis' (s,conf,ws) f,mc'',ms')
+Proof
+  rw[evaluate'_1_ffi_failed, eval_to'_1_Vis] >> simp[SF SFY_ss]
+QED
+
+Theorem eval_to'_1_ffi_evaluate:
+  eval_to' 1 mc ms = (Vis' (s,conf,ws) f,mc',ms') ⇒
+  (∃ms'' ffi'.
+    evaluate' mc (ffi:'ffi ffi_state) 1 ms = (TimeOut,mc',ms'',ffi') ∧ ffi' ≠ ffi) ∨
+  (∃out mc''.  evaluate' mc ffi 1 ms = (Halt (FFI_outcome out),mc'',ms',ffi))
+Proof
+  rw[evaluate'_1_ffi_changed, evaluate'_1_ffi_failed,eval_to'_1_Vis] >>
+  simp[call_FFI_def, AllCaseEqs(), SF DNF_ss] >>
+  Cases_on `ffi.oracle (EL n mc.ffi_names) ffi.ffi_state conf ws` >> simp[]
+QED
+
+
+(*********** trace_prefix **********)
+
+Overload mk_ffi[local] =
+  ``λffi oracle st. ffi with <| oracle := oracle; ffi_state := st |>``;
+
+Triviality mk_ffi_I[simp]:
+  mk_ffi ffi ffi.oracle ffi.ffi_state = ffi
+Proof
+  rw[ffi_state_component_equality]
+QED
+
+Theorem trace_prefix_machine_error:
+  (∃n. trace_prefix n (oracle, ffi_st:'ffi)
+        (machine_sem_itree (mc,ms)) = (io, SOME Error)) ⇔
+  (∃k mc' ms' ffi'.
+    evaluate' mc (mk_ffi ffi oracle ffi_st) k ms = (Error,mc',ms',ffi') ∧
+    ffi'.io_events = ffi.io_events ++ io)
+Proof
+  eq_tac >> rw[] >> rpt $ pop_assum mp_tac
+  >- (
+    map_every qid_spec_tac [`ms`,`mc`,`ffi`,`ffi_st`,`oracle`,`io`,`n`] >>
+    Induct >> rw[trace_prefix_machine_sem_itree] >>
+    pop_assum mp_tac >> TOP_CASE_TAC >> gvs[]
+    >- (
+      rw[] >> gvs[] >> gvs[eval_alt_def] >> every_case_tac >> gvs[] >>
+      pairarg_tac >> gvs[] >>
+      drule $ iffLR eval_to'_evaluate'_error >>
+      disch_then $ qspec_then `mk_ffi ffi oracle ffi_st` assume_tac >> gvs[] >>
+      goal_assum drule >> unabbrev_all_tac >> gvs[]
+      ) >>
+    PairCases_on `e` >> gvs[] >>
+    every_case_tac >> gvs[] >> simp[trace_prefix_def] >>
+    pairarg_tac >> rw[] >> gvs[] >>
+    qpat_x_assum `eval _ = _` mp_tac >> simp[eval_alt_def] >>
+    DEEP_INTRO_TAC some_intro >> rw[] >> gvs[] >> pairarg_tac >> gvs[] >>
+    drule eval_to'_min >> rw[] >> gvs[] >>
+    qpat_x_assum `_ ≤ _` kall_tac >> qpat_x_assum `eval_to' x _ _ = _` kall_tac >>
+    Cases_on `k'` >> gvs[] >> pop_assum $ qspec_then `n'` assume_tac >> gvs[] >>
+    gvs[eval_to'_step_alt] >>
+    drule eval_to'_1_ffi_evaluate >>
+    disch_then $ qspec_then `mk_ffi ffi oracle ffi_st` assume_tac >> reverse $ gvs[]
+    >- (
+      gvs[evaluate'_1_ffi_failed, eval_to'_1_Vis] >>
+      unabbrev_all_tac >> gvs[call_FFI_def, AllCaseEqs()]
+      ) >>
+    drule_all $ iffLR evaluate'_1_ffi_changed >> strip_tac >> gvs[] >>
+    gvs[eval_to'_1_Vis, call_FFI_def, AllCaseEqs()] >>
+    Q.REFINE_EXISTS_TAC `k + SUC n'` >> simp[evaluate'_add, evaluate'_step_alt] >>
+    drule $ iffLR eval_to'_evaluate'_timeout >>
+    disch_then $ qspec_then `mk_ffi ffi oracle ffi_st` assume_tac >> gvs[] >>
+    qmatch_goalsub_abbrev_tac `evaluate' mc0 (mk_ffi ffi0 _ _)` >>
+    last_x_assum drule >> disch_then $ qspec_then `ffi0` assume_tac >> gvs[] >>
+    goal_assum drule >> unabbrev_all_tac >> gvs[]
+    )
+  >- (
+    map_every qid_spec_tac
+      [`ms'`,`mc'`,`ffi'`,`ms`,`mc`,`ffi`,`ffi_st`,`oracle`,`io`,`k`] >>
+    Induct >> rw[evaluate'_step] >>
+    qabbrev_tac `res = evaluate' mc (mk_ffi ffi oracle ffi_st) 1 ms` >>
+    PairCases_on `res` >> gvs[] >> FULL_CASE_TAC >> gvs[]
+    >- (
+      imp_res_tac evaluate'_1_ffi_unchanged >> gvs[] >>
+      gvs[GSYM eval_to'_evaluate'_error] >>
+      simp[machine_sem_itree, eval_alt_def] >>
+      DEEP_INTRO_TAC some_intro >> reverse $ rw[]
+      >- (qexists_tac `1` >> simp[]) >>
+      dxrule eval_to'_agree >> simp[] >> disch_then $ qspec_then `x` $ mp_tac o GSYM >>
+      impl_tac >- metis_tac[PAIR] >> rw[] >> gvs[] >>
+      qexists_tac `SUC n` >> rw[trace_prefix_def]
+      ) >>
+    Cases_on `res3 = mk_ffi ffi oracle ffi_st` >> gvs[]
+    >- (
+      last_x_assum drule >> disch_then drule >> rw[] >>
+      qsuff_tac `eval (mc,ms) = eval (res1,res2)`
+      >- (rw[] >> imp_res_tac machine_sem_itree_eq >> gvs[SF SFY_ss]) >>
+      irule eval_prefix >> gvs[GSYM eval_to'_evaluate'_timeout] >> goal_assum drule
+      ) >>
+    drule_all evaluate'_1_ffi_changed_eval_to' >> rw[] >> gvs[] >>
+    simp[machine_sem_itree, eval_alt_def] >>
+    DEEP_INTRO_TAC some_intro >> reverse $ rw[] >> gvs[]
+    >- (qexists_tac `1` >> simp[]) >>
+    pairarg_tac >> gvs[] >> dxrule_then drule eval_to'_agree >> rw[] >> gvs[] >>
+    drule_all $ iffLR evaluate'_1_ffi_changed >> strip_tac >> gvs[eval_to'_1_Vis] >>
+    gvs[call_FFI_def, AllCaseEqs()] >>
+    Q.REFINE_EXISTS_TAC `SUC m` >> simp[trace_prefix_def] >>
+    gvs[ffi_state_component_equality] >>
+    imp_res_tac evaluate'_io_events_mono >> gvs[io_events_mono_def] >>
+    Cases_on `io` >> gvs[] >>
+    last_x_assum drule >> simp[] >> rw[] >> qexists_tac `n'` >> simp[]
+    )
+QED
+
+Theorem trace_prefix_machine_halt:
+  halt_rel r h ⇒ (
+  (∃n. trace_prefix n (oracle, ffi_st:'ffi)
+        (machine_sem_itree (mc,ms)) = (io, SOME r)) ⇔
+  (∃k mc' ms' ffi'.
+    evaluate' mc (mk_ffi ffi oracle ffi_st) k ms = (Halt h,mc',ms',ffi') ∧
+    ffi'.io_events = ffi.io_events ++ io))
+Proof
+  rw[] >> imp_res_tac halt_rel_imps >> eq_tac >> rw[] >> rpt $ pop_assum mp_tac
+  >- (
+    map_every qid_spec_tac [`ms`,`mc`,`ffi`,`ffi_st`,`oracle`,`io`,`n`] >>
+    Induct >> rw[trace_prefix_machine_sem_itree] >>
+    pop_assum mp_tac >> TOP_CASE_TAC >> gvs[]
+    >- (
+      rw[] >> gvs[] >> gvs[eval_alt_def] >> every_case_tac >> gvs[] >>
+      pairarg_tac >> gvs[] >>
+      drule_all $ iffLR eval_to'_evaluate'_halt_rel >>
+      disch_then $ qspec_then `mk_ffi ffi oracle ffi_st` assume_tac >> gvs[] >>
+      goal_assum drule >> unabbrev_all_tac >> gvs[]
+      ) >>
+    PairCases_on `e` >> gvs[] >>
+    every_case_tac >> gvs[] >> simp[trace_prefix_def] >>
+    pairarg_tac >> rw[] >> gvs[] >>
+    qpat_x_assum `eval _ = _` mp_tac >> simp[eval_alt_def] >>
+    DEEP_INTRO_TAC some_intro >> rw[] >> gvs[] >> pairarg_tac >> gvs[] >>
+    drule eval_to'_min >> rw[] >> gvs[] >>
+    qpat_x_assum `_ ≤ _` kall_tac >> qpat_x_assum `eval_to' x _ _ = _` kall_tac >>
+    Cases_on `k'` >> gvs[] >> pop_assum $ qspec_then `n'` assume_tac >> gvs[] >>
+    gvs[eval_to'_step_alt] >>
+    drule eval_to'_1_ffi_evaluate >>
+    disch_then $ qspec_then `mk_ffi ffi oracle ffi_st` assume_tac >> reverse $ gvs[]
+    >- (
+      gvs[evaluate'_1_ffi_failed, eval_to'_1_Vis] >>
+      unabbrev_all_tac >> gvs[call_FFI_def, AllCaseEqs()]
+      ) >>
+    drule_all $ iffLR evaluate'_1_ffi_changed >> strip_tac >> gvs[] >>
+    gvs[eval_to'_1_Vis, call_FFI_def, AllCaseEqs()] >>
+    Q.REFINE_EXISTS_TAC `k + SUC n'` >> simp[evaluate'_add, evaluate'_step_alt] >>
+    drule $ iffLR eval_to'_evaluate'_timeout >>
+    disch_then $ qspec_then `mk_ffi ffi oracle ffi_st` assume_tac >> gvs[] >>
+    qmatch_goalsub_abbrev_tac `evaluate' mc0 (mk_ffi ffi0 _ _)` >>
+    last_x_assum drule >> disch_then $ qspec_then `ffi0` assume_tac >> gvs[] >>
+    goal_assum drule >> unabbrev_all_tac >> gvs[]
+    )
+  >- (
+    map_every qid_spec_tac
+      [`ms'`,`mc'`,`ffi'`,`ms`,`mc`,`ffi`,`ffi_st`,`oracle`,`io`,`k`] >>
+    Induct >> rw[evaluate'_step] >>
+    qabbrev_tac `res = evaluate' mc (mk_ffi ffi oracle ffi_st) 1 ms` >>
+    PairCases_on `res` >> gvs[] >> FULL_CASE_TAC >> gvs[]
+    >- (
+      imp_res_tac evaluate'_1_ffi_unchanged >> gvs[] >>
+      drule $ GSYM eval_to'_evaluate'_halt_rel >> disch_then $ gvs o single >>
+      simp[machine_sem_itree, eval_alt_def] >>
+      DEEP_INTRO_TAC some_intro >> reverse $ rw[]
+      >- (qexists_tac `1` >> simp[]) >>
+      dxrule eval_to'_agree >> simp[] >> disch_then $ qspec_then `x` $ mp_tac o GSYM >>
+      impl_tac >- metis_tac[PAIR] >> rw[] >> gvs[] >>
+      qexists_tac `SUC n` >> rw[trace_prefix_def]
+      ) >>
+    Cases_on `res3 = mk_ffi ffi oracle ffi_st` >> gvs[]
+    >- (
+      last_x_assum drule >> disch_then drule >> rw[] >>
+      qsuff_tac `eval (mc,ms) = eval (res1,res2)`
+      >- (rw[] >> imp_res_tac machine_sem_itree_eq >> gvs[SF SFY_ss]) >>
+      irule eval_prefix >> gvs[GSYM eval_to'_evaluate'_timeout] >> goal_assum drule
+      ) >>
+    drule_all evaluate'_1_ffi_changed_eval_to' >> rw[] >> gvs[] >>
+    simp[machine_sem_itree, eval_alt_def] >>
+    DEEP_INTRO_TAC some_intro >> reverse $ rw[] >> gvs[]
+    >- (qexists_tac `1` >> simp[]) >>
+    pairarg_tac >> gvs[] >> dxrule_then drule eval_to'_agree >> rw[] >> gvs[] >>
+    drule_all $ iffLR evaluate'_1_ffi_changed >> strip_tac >> gvs[eval_to'_1_Vis] >>
+    gvs[call_FFI_def, AllCaseEqs()] >>
+    Q.REFINE_EXISTS_TAC `SUC m` >> simp[trace_prefix_def] >>
+    gvs[ffi_state_component_equality] >>
+    imp_res_tac evaluate'_io_events_mono >> gvs[io_events_mono_def] >>
+    Cases_on `io` >> gvs[] >>
+    last_x_assum drule >> simp[] >> rw[] >> qexists_tac `n'` >> simp[]
+    )
+QED
+
+Theorem trace_prefix_machine_ffi_error:
+  (∃n. trace_prefix n (oracle, ffi_st:'ffi)
+        (machine_sem_itree (mc,ms)) = (io, SOME (FinalFFI (s,conf,ws) out))) ⇔
+  (∃k mc' ms' ffi'.
+    evaluate' mc (mk_ffi ffi oracle ffi_st) k ms =
+      (Halt (FFI_outcome (Final_event s conf ws out)),mc',ms',ffi') ∧
+    ffi'.io_events = ffi.io_events ++ io)
+Proof
+  rw[] >> imp_res_tac halt_rel_imps >> eq_tac >> rw[] >> rpt $ pop_assum mp_tac
+  >- (
+    map_every qid_spec_tac [`ms`,`mc`,`ffi`,`ffi_st`,`oracle`,`io`,`n`] >>
+    Induct >> rw[trace_prefix_machine_sem_itree] >>
+    pop_assum mp_tac >> TOP_CASE_TAC >> gvs[]
+    >- (
+      rw[] >> gvs[] >> gvs[eval_alt_def] >> every_case_tac >> gvs[] >>
+      pairarg_tac >> gvs[eval_to'_Ret_FinalFFI]
+      ) >>
+    PairCases_on `e` >> gvs[] >>
+    every_case_tac >> gvs[] >> rw[trace_prefix_def] >> gvs[] >>
+    qpat_x_assum `eval _ = _` mp_tac >> simp[eval_alt_def] >>
+    DEEP_INTRO_TAC some_intro >> rw[] >> gvs[] >> pairarg_tac >> gvs[] >>
+    drule eval_to'_min >> rw[] >> gvs[] >>
+    qpat_x_assum `_ ≤ _` kall_tac >> qpat_x_assum `eval_to' x _ _ = _` kall_tac >>
+    Cases_on `k'` >> gvs[] >> pop_assum $ qspec_then `n'` assume_tac >> gvs[] >>
+    gvs[eval_to'_step_alt] >>
+    drule eval_to'_1_ffi_evaluate >>
+    disch_then $ qspec_then `mk_ffi ffi oracle ffi_st` assume_tac >> reverse $ gvs[]
+    >- (
+      qexists_tac `SUC n'` >> simp[evaluate'_step_alt] >>
+      drule $ iffLR eval_to'_evaluate'_timeout >>
+      disch_then $ qspec_then `mk_ffi ffi oracle ffi_st` assume_tac >> simp[] >>
+      gvs[evaluate'_1_ffi_failed, eval_to'_1_Vis] >>
+      unabbrev_all_tac >> gvs[call_FFI_def, AllCaseEqs()]
+      )
+    >- (
+      drule_all $ iffLR evaluate'_1_ffi_changed >> rw[] >> gvs[] >>
+      gvs[call_FFI_def, AllCaseEqs(), eval_to'_1_Vis]
+      )
+    >- (
+      qexists_tac `SUC n'` >> simp[evaluate'_step_alt] >>
+      drule $ iffLR eval_to'_evaluate'_timeout >>
+      disch_then $ qspec_then `mk_ffi ffi oracle ffi_st` assume_tac >> simp[] >>
+      gvs[evaluate'_1_ffi_failed, eval_to'_1_Vis] >>
+      unabbrev_all_tac >> gvs[call_FFI_def, AllCaseEqs()]
+      )
+    >- (
+      pairarg_tac >> gvs[] >> rename [`Div',mc1,ms1`,`Vis' _ _,mc2,ms2`] >>
+      drule $ iffLR eval_to'_evaluate'_timeout >>
+      disch_then $ qspec_then `mk_ffi ffi oracle ffi_st` assume_tac >>
+      Q.REFINE_EXISTS_TAC `SUC n' + k` >>
+      simp[evaluate'_add_alt, evaluate'_step_alt] >>
+      drule_all $ iffLR evaluate'_1_ffi_changed >> rw[] >> gvs[] >>
+      gvs[call_FFI_def, AllCaseEqs(), eval_to'_1_Vis, ffi_state_component_equality] >>
+      qmatch_goalsub_abbrev_tac `evaluate' mc1' _ _ ms1'` >>
+      last_x_assum drule >> disch_then $ qspec_then `ffi'` assume_tac >> gvs[SF SFY_ss]
+      )
+    >- (
+      qexists_tac `SUC n'` >> simp[evaluate'_step_alt] >>
+      drule $ iffLR eval_to'_evaluate'_timeout >>
+      disch_then $ qspec_then `mk_ffi ffi oracle ffi_st` assume_tac >> simp[] >>
+      gvs[evaluate'_1_ffi_failed, eval_to'_1_Vis] >>
+      unabbrev_all_tac >> gvs[call_FFI_def, AllCaseEqs()]
+      )
+    >- (
+      drule_all $ iffLR evaluate'_1_ffi_changed >> rw[] >> gvs[] >>
+      gvs[call_FFI_def, AllCaseEqs(), eval_to'_1_Vis]
+      )
+    )
+  >- (
+    map_every qid_spec_tac
+      [`ms'`,`mc'`,`ffi'`,`ms`,`mc`,`ffi`,`ffi_st`,`oracle`,`io`,`k`] >>
+    Induct >> rw[evaluate'_step] >>
+    qabbrev_tac `res = evaluate' mc (mk_ffi ffi oracle ffi_st) 1 ms` >>
+    PairCases_on `res` >> gvs[] >> FULL_CASE_TAC >> gvs[]
+    >- (
+      imp_res_tac evaluate'_1_ffi_failed_eval_to' >>
+      gvs[evaluate'_1_ffi_failed, call_FFI_def, AllCaseEqs()] >>
+      simp[machine_sem_itree, eval_alt_def] >>
+      (DEEP_INTRO_TAC some_intro >> reverse $ rw[] >- (qexists_tac `1` >> simp[])) >>
+      pairarg_tac >> gvs[] >>
+      dxrule_then drule eval_to'_agree >> rw[] >> gvs[] >>
+      qexists_tac `SUC (SUC n)` >> gvs[eval_to'_1_Vis, trace_prefix_def]
+      ) >>
+    Cases_on `res3 = mk_ffi ffi oracle ffi_st` >> gvs[]
+    >- (
+      last_x_assum drule >> disch_then drule >> rw[] >>
+      qsuff_tac `eval (mc,ms) = eval (res1,res2)`
+      >- (rw[] >> imp_res_tac machine_sem_itree_eq >> gvs[SF SFY_ss]) >>
+      irule eval_prefix >> gvs[GSYM eval_to'_evaluate'_timeout] >> goal_assum drule
+      ) >>
+    drule_all evaluate'_1_ffi_changed_eval_to' >> rw[] >> gvs[] >>
+    simp[machine_sem_itree, eval_alt_def] >>
+    DEEP_INTRO_TAC some_intro >> reverse $ rw[] >> gvs[]
+    >- (qexists_tac `1` >> simp[]) >>
+    pairarg_tac >> gvs[] >> dxrule_then drule eval_to'_agree >> rw[] >> gvs[] >>
+    drule_all $ iffLR evaluate'_1_ffi_changed >> strip_tac >> gvs[eval_to'_1_Vis] >>
+    gvs[call_FFI_def, AllCaseEqs()] >>
+    Q.REFINE_EXISTS_TAC `SUC m` >> simp[trace_prefix_def] >>
+    gvs[ffi_state_component_equality] >>
+    imp_res_tac evaluate'_io_events_mono >> gvs[io_events_mono_def] >>
+    Cases_on `io` >> gvs[] >>
+    last_x_assum drule >> simp[] >> rw[] >> qexists_tac `n'` >> simp[]
+    )
+QED
+
+Theorem trace_prefix_evaluate'_io_events:
+  ∀n oracle ffi ffi_st mc ms io.
+    trace_prefix n (oracle, ffi_st:'ffi)
+      (machine_sem_itree (mc,ms)) = (io, NONE)
+  ⇒ ∃k mc' ms' ffi'.
+      evaluate' mc (mk_ffi ffi oracle ffi_st) k ms =
+        (TimeOut,mc',ms',ffi') ∧
+      ffi'.io_events = ffi.io_events ++ io
+Proof
+  Induct >> rw[trace_prefix_def] >- (qexists_tac `0` >> simp[]) >>
+  gvs[trace_prefix_machine_sem_itree, eval_alt_def] >>
+  pop_assum mp_tac >> DEEP_INTRO_TAC some_intro >> reverse $ rw[]
+  >- (qexists_tac `0` >> simp[]) >>
+  pop_assum mp_tac >> pairarg_tac >> gvs[] >>
+  TOP_CASE_TAC >> gvs[] >> PairCases_on `e` >> gvs[] >>
+  every_case_tac >> rw[] >> gvs[]
+  >- (qexists_tac `0` >> simp[])
+  >- (
+    gvs[trace_prefix_def] >>
+    drule eval_to'_min >> rw[] >> gvs[] >>
+    qpat_x_assum `_ ≤ _` kall_tac >> qpat_x_assum `eval_to' x _ _ = _` kall_tac >>
+    Cases_on `k'` >> gvs[] >> pop_assum $ qspec_then `n` assume_tac >> gvs[] >>
+    gvs[eval_to'_step_alt] >>
+    drule $ iffLR eval_to'_evaluate'_timeout >>
+    disch_then $ qspec_then `mk_ffi ffi oracle ffi_st` assume_tac >>
+    qexists_tac `SUC n` >> simp[evaluate'_step_alt] >>
+    drule eval_to'_1_ffi_evaluate >>
+    disch_then $ qspec_then `mk_ffi ffi oracle ffi_st` assume_tac >> reverse $ gvs[]
+    >- gvs[evaluate'_1_ffi_failed, eval_to'_1_Vis, call_FFI_def] >>
+    drule_all $ iffLR evaluate'_1_ffi_changed >> rw[] >> gvs[] >>
+    gvs[eval_to'_1_Vis, call_FFI_def]
+    )
+  >- (qexists_tac `0` >> simp[])
+  >- (
+    pairarg_tac >> gvs[] >>
+    drule eval_to'_min >> rw[] >> gvs[] >>
+    qpat_x_assum `_ ≤ _` kall_tac >> qpat_x_assum `eval_to' x _ _ = _` kall_tac >>
+    Cases_on `k'` >> gvs[] >> pop_assum $ qspec_then `n'` assume_tac >> gvs[] >>
+    gvs[eval_to'_step_alt] >>
+    drule $ iffLR eval_to'_evaluate'_timeout >>
+    disch_then $ qspec_then `mk_ffi ffi oracle ffi_st` assume_tac >>
+    Q.REFINE_EXISTS_TAC `SUC n' + k` >>
+    simp[evaluate'_add_alt, evaluate'_step_alt] >>
+    drule eval_to'_1_ffi_evaluate >>
+    disch_then $ qspec_then `mk_ffi ffi oracle ffi_st` assume_tac >> reverse $ gvs[]
+    >- gvs[evaluate'_1_ffi_failed, eval_to'_1_Vis, call_FFI_def] >>
+    drule_all $ iffLR evaluate'_1_ffi_changed >> rw[] >> gvs[] >>
+    gvs[eval_to'_1_Vis, call_FFI_def] >>
+    qmatch_goalsub_abbrev_tac `mk_ffi ffi0 _ _` >>
+    last_x_assum drule >> disch_then $ qspec_then `ffi0` assume_tac >> gvs[] >>
+    goal_assum drule >> unabbrev_all_tac >> gvs[]
+    )
+QED
+
+Theorem evaluate'_trace_prefix_io_events:
+  ∀k mc (ffi:'ffi ffi_state) ms mc' ms' ffi'.
+    evaluate' mc ffi k ms = (TimeOut,mc',ms',ffi')
+  ⇒ ∃n io.
+      trace_prefix n (ffi.oracle,ffi.ffi_state)
+        (machine_sem_itree (mc,ms)) = (io,NONE) ∧
+      ffi'.io_events = ffi.io_events ++ io
+Proof
+  Induct >> rw[evaluate'_step] >- (qexists_tac `0` >> rw[trace_prefix_def]) >>
+  qabbrev_tac `res = evaluate' mc ffi 1 ms` >> PairCases_on `res` >> gvs[] >>
+  Cases_on `res0` >> gvs[] >> Cases_on `res3 = ffi` >> gvs[]
+  >- (
+    last_x_assum drule >> rw[] >>
+    qsuff_tac `eval (mc,ms) = eval (res1,res2)`
+    >- (rw[] >> imp_res_tac machine_sem_itree_eq >> gvs[SF SFY_ss]) >>
+    irule eval_prefix >> gvs[GSYM eval_to'_evaluate'_timeout] >> goal_assum drule
+    ) >>
+  drule_all evaluate'_1_ffi_changed_eval_to' >> rw[] >> gvs[] >>
+  simp[machine_sem_itree, eval_alt_def] >>
+  DEEP_INTRO_TAC some_intro >> reverse $ rw[]
+  >- (pop_assum $ qspec_then `1` assume_tac >> gvs[]) >>
+  pairarg_tac >> gvs[] >> dxrule_then drule eval_to'_agree >> rw[] >> gvs[] >>
+  drule_all $ iffLR evaluate'_1_ffi_changed >> strip_tac >> gvs[eval_to'_1_Vis] >>
+  gvs[call_FFI_def, AllCaseEqs()] >>
+  Q.REFINE_EXISTS_TAC `SUC m` >> simp[trace_prefix_def] >>
+  gvs[ffi_state_component_equality] >>
+  last_x_assum drule >> rw[] >> qexists_tac `n'` >> simp[]
+QED
+
+Theorem evaluate'_trace_prefix_diverge:
+  (∀n. ∃io. trace_prefix n (oracle,ffi_st:'ffi)
+    (machine_sem_itree (mc,ms)) = (io,NONE)) ⇔
+  (∀k. ∃mc' ms' ffi'.
+    evaluate' mc (mk_ffi ffi oracle ffi_st) k ms = (TimeOut,mc',ms',ffi'))
+Proof
+  eq_tac >> rw[]
+  >- (
+    CCONTR_TAC >> gvs[] >>
+    qabbrev_tac `res = evaluate' mc (mk_ffi ffi oracle ffi_st) k ms` >>
+    PairCases_on `res` >> gvs[] >> imp_res_tac evaluate'_io_events_mono >>
+    gvs[io_events_mono_def, IS_PREFIX_APPEND] >>
+    reverse $ Cases_on `res0` >> gvs[]
+    >- (
+      drule_all $ SRULE [PULL_EXISTS] $ iffRL trace_prefix_machine_error >>
+      strip_tac >> gvs[] >> last_x_assum $ qspec_then `n` mp_tac >> simp[]
+      ) >>
+    Cases_on `∃h. halt_rel h o'` >> gvs[]
+    >- (
+      drule_all $ SRULE [PULL_EXISTS] $ iffRL trace_prefix_machine_halt >>
+      strip_tac >> gvs[] >> last_x_assum $ qspec_then `n` mp_tac >> simp[]
+      ) >>
+    Cases_on `o'` >> gvs[halt_rel_alt_def] >> Cases_on `f` >>
+    drule_all $ SRULE [PULL_EXISTS] $ iffRL trace_prefix_machine_ffi_error >>
+    strip_tac >> gvs[] >> last_x_assum $ qspec_then `n` mp_tac >> simp[]
+    )
+  >- (
+    CCONTR_TAC >> gvs[] >>
+    Cases_on `trace_prefix n (oracle,ffi_st) (machine_sem_itree (mc,ms))` >> gvs[] >>
+    Cases_on `r` >> gvs[] >> Cases_on `x` >> gvs[]
+    >- (
+      `halt_rel Termination Success` by gvs[halt_rel_def] >>
+      drule_all $ SRULE [PULL_EXISTS] $ iffLR trace_prefix_machine_halt >>
+      disch_then $ qspec_then `ffi` assume_tac >> gvs[] >>
+      last_x_assum $ qspec_then `k` assume_tac >> gvs[]
+      )
+    >- (
+      `halt_rel OutOfMemory Resource_limit_hit` by gvs[halt_rel_def] >>
+      drule_all $ SRULE [PULL_EXISTS] $ iffLR trace_prefix_machine_halt >>
+      disch_then $ qspec_then `ffi` assume_tac >> gvs[] >>
+      last_x_assum $ qspec_then `k` assume_tac >> gvs[]
+      )
+    >- (
+      drule_all $ SRULE [PULL_EXISTS] $ iffLR trace_prefix_machine_error >>
+      disch_then $ qspec_then `ffi` assume_tac >> gvs[] >>
+      last_x_assum $ qspec_then `k` assume_tac >> gvs[]
+      )
+    >- (
+      PairCases_on `p` >>
+      drule_all $ SRULE [PULL_EXISTS] $ iffLR trace_prefix_machine_ffi_error >>
+      disch_then $ qspec_then `ffi` assume_tac >> gvs[] >>
+      last_x_assum $ qspec_then `k` assume_tac >> gvs[]
+      )
+    )
+QED
+
+Triviality trace_prefix_machine_halt_alt =
+  Q.INST [`oracle` |-> `ffi.oracle`, `ffi_st` |-> `ffi.ffi_state`]
+    trace_prefix_machine_halt |> SRULE [];
+
+Triviality trace_prefix_machine_error_alt =
+  Q.INST [`oracle` |-> `ffi.oracle`, `ffi_st` |-> `ffi.ffi_state`]
+    trace_prefix_machine_error |> SRULE [];
+
+Triviality trace_prefix_machine_ffi_error_alt =
+  Q.INST [`oracle` |-> `ffi.oracle`, `ffi_st` |-> `ffi.ffi_state`]
+    trace_prefix_machine_ffi_error |> SRULE [];
+
+Theorem lprefix_chain_evaluate':
+  lprefix_chain
+    (IMAGE (λk. fromList (SND (SND (SND (evaluate' mc st k ms)))).io_events) 𝕌(:num))
+Proof
+  rw[lprefix_chain_def] >> simp[LPREFIX_fromList, from_toList] >>
+  wlog_tac `k ≤ k'` [`k`,`k'`] >- (`k' ≤ k` by gvs[] >> metis_tac[]) >>
+  disj1_tac >> imp_res_tac LESS_EQUAL_ADD >> gvs[] >>
+  simp[evaluate'_add_alt] >>
+  qabbrev_tac `res = evaluate' mc st k ms` >> PairCases_on `res` >> gvs[] >>
+  CASE_TAC >> gvs[] >>
+  qpat_abbrev_tac `res' = evaluate' _ _ _ _` >> PairCases_on `res'` >> gvs[] >>
+  imp_res_tac evaluate'_io_events_mono >> gvs[io_events_mono_def]
+QED
+
+Theorem itree_machine_semantics:
+  (machine_sem mc (ffi:'ffi ffi_state) ms (Terminate outcome io_list) ⇔
+    ∃n io res.
+      trace_prefix n (ffi.oracle, ffi.ffi_state)
+        (machine_sem_itree (mc,ms)) = (io, SOME res) ∧
+      io_list = ffi.io_events ++ io ∧
+      if outcome = Success then res = Termination
+      else if outcome = Resource_limit_hit then res = OutOfMemory
+      else ∃s conf ws f.
+              outcome = FFI_outcome (Final_event s conf ws f) ∧
+              res = FinalFFI (s,conf,ws) f) ∧
+
+  (machine_sem mc ffi ms (Diverge io_trace) ⇔
+    (∀n. ∃io. trace_prefix n (ffi.oracle, ffi.ffi_state)
+                (machine_sem_itree (mc,ms)) = (io, NONE)) ∧
+    lprefix_lub
+      { fromList (ffi.io_events ++ io) | io |
+          ∃n res. trace_prefix n (ffi.oracle, ffi.ffi_state)
+                    (machine_sem_itree (mc,ms)) = (io, res) }
+      io_trace) ∧
+
+  (machine_sem mc ffi ms Fail ⇔
+    ∃n io. trace_prefix n (ffi.oracle, ffi.ffi_state)
+            (machine_sem_itree (mc,ms)) = (io, SOME Error))
+Proof
+  rw[machine_sem_def, evaluate_evaluate']
+  >- ( (* termination *)
+    Cases_on `∃h. halt_rel h outcome` >> gvs[]
+    >- (
+      eq_tac >> rw[]
+      >- (
+        pairarg_tac >> gvs[] >> imp_res_tac evaluate'_io_events_mono >>
+        gvs[io_events_mono_def, IS_PREFIX_APPEND] >>
+        drule_all $ SRULE [PULL_EXISTS] $ iffRL trace_prefix_machine_halt_alt >>
+        strip_tac >> goal_assum drule >>
+        Cases_on `h` >> gvs[halt_rel_def]
+        )
+      >- (
+        `res = h` by (Cases_on `h` >> gvs[halt_rel_def]) >> gvs[] >>
+        drule_all $ SRULE [PULL_EXISTS] $ iffLR trace_prefix_machine_halt_alt >>
+        rw[] >> qexists_tac `k` >> simp[]
+        )
+      )
+    >- (
+      Cases_on `outcome` >> gvs[halt_rel_alt_def] >> eq_tac >> rw[]
+      >- (
+        pairarg_tac >> gvs[] >> imp_res_tac evaluate'_io_events_mono >>
+        gvs[io_events_mono_def, IS_PREFIX_APPEND] >> Cases_on `f` >>
+        drule_all $ SRULE [PULL_EXISTS] $ iffRL trace_prefix_machine_ffi_error_alt >>
+        strip_tac >> goal_assum drule >> simp[]
+        )
+      >- (
+        drule_all $ SRULE [PULL_EXISTS] $ iffLR trace_prefix_machine_ffi_error_alt >>
+        rw[] >> qexists_tac `k` >> simp[]
+        )
+      )
+    )
+  >- ( (* divergence *)
+    irule $ DECIDE ``a = c ∧ (a ∧ c ⇒ b = d) ⇒ (a ∧ b ⇔ c ∧ d)`` >> rw[]
+    >- (
+      eq_tac >> rw[]
+      >- (
+        irule $ iffRL evaluate'_trace_prefix_diverge >> qexists_tac `ffi` >> rw[] >>
+        pop_assum $ qspec_then `k` assume_tac >> pairarg_tac >> gvs[]
+        )
+      >- (
+        pairarg_tac >> gvs[] >> drule $ iffLR evaluate'_trace_prefix_diverge >>
+        disch_then $ qspecl_then [`ffi`,`k`] assume_tac >> gvs[]
+        )
+      ) >>
+    irule lprefix_lub_equiv_chain >> irule_at Any IMP_equiv_lprefix_chain >>
+    simp[UNCURRY, lprefix_chain_trace_prefix, lprefix_chain_evaluate'] >>
+    rw[lprefix_rel_def, PULL_EXISTS, LPREFIX_fromList, from_toList]
+    >- (
+      last_x_assum $ qspec_then `k` assume_tac >> pairarg_tac >> gvs[] >>
+      drule evaluate'_trace_prefix_io_events >> rw[] >> goal_assum drule >> simp[]
+      )
+    >- (
+      first_x_assum $ qspec_then `n` assume_tac >> gvs[] >>
+      drule trace_prefix_evaluate'_io_events >>
+      disch_then $ qspec_then `ffi` assume_tac >> gvs[] >> qexists_tac `k` >> simp[]
+      )
+    )
+  >- ( (* type error *)
+    eq_tac >> rw[]
+    >- (
+      pairarg_tac >> gvs[] >> imp_res_tac evaluate'_io_events_mono >>
+      gvs[io_events_mono_def, IS_PREFIX_APPEND] >>
+      drule_all $ SRULE [PULL_EXISTS] $ iffRL trace_prefix_machine_error_alt >>
+      strip_tac >> goal_assum drule
+      )
+    >- (
+      drule_all $ SRULE [PULL_EXISTS] $ iffLR trace_prefix_machine_error_alt >>
+      rw[] >> qexists_tac `k` >> simp[]
+      )
+    )
+QED
+
+
 (**********)
 
 val _ = export_theory();
